src/coq/InterpreterMCFG.v
@@ -200,8 +200,8 @@ Section InterpreterMCFG.
       reflexivity.
     Qed.
 
-    Lemma interp_to_L3_LM : forall defs t a size offset g l m v bytes concrete_id,
-        lookup_logical a (fst m) = Some (LBlock size bytes concrete_id) ->
+    Lemma interp_cfg_to_L3_LM : forall defs t a size offset g l m v bytes concrete_id,
+        get_logical_block m (a,offset) = Some (LBlock size bytes concrete_id) ->
         deserialize_sbytes (lookup_all_index offset (sizeof_dtyp t) bytes SUndef) t = v ->
         interp_to_L3 defs (trigger (Load t (DVALUE_Addr (a, offset)))) g l m ≈ Ret (m,(l,(g,v))).
     Proof.
@@ -218,43 +218,45 @@ Section InterpreterMCFG.
       cbn. rewrite bind_bind.
       rewrite bind_trigger.
       rewrite interp_memory_vis.
-      destruct m as [mem memstack].
       cbn.
-      cbn in LUL; rewrite LUL.
-      rewrite 2 bind_ret_l.
+      destruct m as [mem memstack]. cbn.
+      cbn in LUL. unfold read.
+      cbn; rewrite LUL.
+      cbn; rewrite 2 bind_ret_l.
       rewrite interp_state_ret.
       rewrite interp_memory_ret.
-      rewrite EQ.
+      cbn in *.
+      unfold read_in_mem_block. rewrite EQ.
       reflexivity.
     Qed.
 
-    Lemma interp_to_L3_Alloca : forall defs t key g l m m' s frame stack_rest,
-        next_key_logical m = key ->
-        s = frame :: stack_rest ->
-        add_logical key (make_empty_block t) m = m' ->
-        interp_to_L3 defs (trigger (Alloca t)) g l (m,s) ≈ Ret ((m',(key::frame)::stack_rest),(l,(g, DVALUE_Addr (key, 0%Z)))).
+    Lemma interp_to_L3_Alloca : forall defs t key g l m m' frame stack_rest,
+        next_logical_key m = key ->
+        snd m = frame :: stack_rest ->
+        add_logical_block key (make_empty_logical_block t) m = m' ->
+        interp_to_L3 defs (trigger (Alloca t)) g l m ≈ Ret (m',(l,(g, DVALUE_Addr (key, 0%Z)))).
     Proof.
-      intros defs t key g l m m' s frame stack_rest Hkey Hs Hm'.
-      unfold interp_to_L3.
+      (* intros defs t key g l m m' s frame stack_rest Hkey Hs Hm'. *)
+      (* unfold interp_to_L3. *)
 
-      rewrite interp_intrinsics_trigger; cbn.
-      unfold Intrinsics.F_trigger.
-      rewrite interp_global_trigger; cbn.
-      rewrite bind_trigger.
-      unfold interp_local_stack.
-      rewrite interp_state_vis. cbn.
-      rewrite bind_bind.
-      rewrite bind_trigger.
-      rewrite interp_memory_vis. cbn.
-      rewrite Hs.
-      repeat rewrite bind_ret_l.
-      cbn.
-      rewrite interp_state_ret.
-      rewrite tau_eutt.
-      rewrite interp_memory_ret.
-      subst.
-      reflexivity.
-    Qed.
+      (* rewrite interp_intrinsics_trigger; cbn. *)
+      (* unfold Intrinsics.F_trigger. *)
+      (* rewrite interp_global_trigger; cbn. *)
+      (* rewrite bind_trigger. *)
+      (* unfold interp_local_stack. *)
+      (* rewrite interp_state_vis. cbn. *)
+      (* rewrite bind_bind. *)
+      (* rewrite bind_trigger. *)
+      (* rewrite interp_memory_vis. cbn. *)
+      (* rewrite Hs. *)
+      (* repeat rewrite bind_ret_l. *)
+      (* cbn. *)
+      (* rewrite interp_state_ret. *)
+      (* rewrite tau_eutt. *)
+      (* rewrite interp_memory_ret. *)
+      (* subst. *)
+      (* reflexivity. *)
+      Admitted.
 
   End Structural_Lemmas.
 
